## Question 3

Put the following expressions into beta normal form (use β-reduction as far as possible, α-conversion as needed) assuming left-association.
```
1. (λz.z) (λq.q q) (λs.s a)
= (λz.z) (q) [q->q] (s)[s->a]
= (λz.z) q a
= (z) [z->q] a
= q a

```

```
2. (λz.z) (λz.z z) (λz.z q)
= {(λz.z) (λz'.z' z')} (λz.z q)
= {(λz.z) (z' [z'->z'])} (λz.z q)
= {(λz.z) (z')} (λz.z q)
= {(z) [z->z']} (λz.z q)
= (z') (λz.z q)
= (z') (z [z->q])
= z' q

```

```
3. (λs.λq.s q q) (λa.a) b
= (λs.(λq.s q q)) (λa.a) b
= (λs.(s [q->q] q)) (λa.a) b
= (λs.(s q)) (λa.a) b
= (s [s->q]) (λa.a) b
= (q) (λa.a) b
= (q) (a [a->b])
= q b

```

```
4. (λs.λq.s q q) (λq.q) q
= (λs.(λq.s q q)) (λq.q) q
= (λs.(s [q->q] q)) (λq.q) q
= (λs.(s q)) (λq.q) q
= (s [s->q]) (λq.q) q
= (q) (λq'.q') q'
= (q) (q') [q'->q']
= q q'

```

```
5. ((λs.s s) (λq.q)) (λq.q)
= ((s [s->s]) (λq.q)) (λq.q)
= ((s) (λq.q)) (λq.q)
= (s) q [q-> (λq'.q')]
= s (λq'.q')

```